Splinter/GCLayer/GCCrashTolerantJournalRefinement.i.dfy
@@ -1,0 +1,148 @@
+// Copyright 2018-2021 VMware, Inc., Microsoft Inc., Carnegie Mellon University, ETH Zurich, and University of Washington
+// SPDX-License-Identifier: BSD-2-Clause
+
+include "GCCrashTolerantJournal.i.dfy"
+include "../CoordinationLayer/AbstractJournal.i.dfy"
+include "../CoordinationLayer/CrashTolerantJournal.i.dfy"
+include "../Journal/PagedJournalRefinement.i.dfy"
+include "../Journal/LinkedJournalRefinement.i.dfy"
+include "../Journal/ReprJournalRefinement.i.dfy"
+
+module GCCrashTolerantJournalRefinement {
+  import opened Options
+  import AbstractJournal
+  import PagedJournalRefinement
+  import LinkedJournalRefinement
+  import ReprJournalRefinement
+  import CrashTolerantJournal 
+  import opened GCCrashTolerantJournal
+
+  function IALabel(lbl: TransitionLabel) : CrashTolerantJournal.TransitionLabel
+  {
+    lbl.base
+  }
+
+  function IImage(image: StoreImage) : CrashTolerantJournal.StoreImage 
+    requires image.WF()
+  {
+    // turn GCTruncatedJournal to msgHistory
+    PagedJournalRefinement.ITruncatedJournal(LinkedJournalRefinement.ITruncatedJournal(image.journal))
+  }
+
+  function IReprJ(rj: ReprJournal.Variables) : AbstractJournal.Variables
+    requires rj.WF()
+    requires rj.journal.truncatedJournal.Decodable()
+  {
+    PagedJournalRefinement.I(LinkedJournalRefinement.I(ReprJournalRefinement.I(rj)))
+  }
+
+  function I(v: Variables) : CrashTolerantJournal.Variables
+    requires v.WF()
+    requires v.ephemeral.Known? ==> v.ephemeral.v.journal.truncatedJournal.Decodable()
+  {
+    CrashTolerantJournal.Variables(
+      IImage(v.persistent),
+      if v.ephemeral.Unknown?  then CrashTolerantJournal.Unknown else CrashTolerantJournal.Known(IReprJ(v.ephemeral.v)),
+      if v.inFlight.None? then None else Some(IImage(v.inFlight.value))
+    )
+  }
+
+  predicate Inv(v: Variables) {
+    && v.WF()
+    && (v.ephemeral.Known? ==> 
+          && v.ephemeral.v.journal.truncatedJournal.Decodable()
+          && ReprJournalRefinement.Inv(v.ephemeral.v)
+      )
+  }
+
+  lemma InitRefines(v: Variables)
+    requires Inv(v)
+    requires Init(v)
+    ensures Inv(v)
+    ensures CrashTolerantJournal.Init(I(v))
+  {}
+
+  lemma LoadEphemeralFromPersistentRefines(v: Variables, v': Variables, lbl: TransitionLabel)
+    requires Inv(v)
+    requires Next(v, v', lbl)
+    requires lbl.base.LoadEphemeralFromPersistentLabel?
+    ensures Inv(v') 
+    ensures CrashTolerantJournal.Next(I(v), I(v'), IALabel(lbl))
+  {
+    ReprJournalRefinement.InvInit(v'.ephemeral.v, v.persistent);
+  }
+
+  lemma ReadForRecoveryRefines(v: Variables, v': Variables, lbl: TransitionLabel)
+    requires Inv(v)
+    requires Next(v, v', lbl) 
+    requires lbl.base.ReadForRecoveryLabel?
+    ensures Inv(v')
+    ensures CrashTolerantJournal.Next(I(v), I(v'), IALabel(lbl))
+  {
+    var j, j' := v.ephemeral.v, v'.ephemeral.v;
+    var jLbl := ReprJournal.ReadForRecoveryLabel(lbl.base.records);
+    ReprJournalRefinement.NextRefines(j, j', jLbl);
+    LinkedJournalRefinement.NextRefines(
+      ReprJournalRefinement.I(j),
+      ReprJournalRefinement.I(j'),
+      jLbl.I());
+    PagedJournalRefinement.NextRefines(
+      LinkedJournalRefinement.I(ReprJournalRefinement.I(j)),
+      LinkedJournalRefinement.I(ReprJournalRefinement.I(j')),
+      LinkedJournalRefinement.ILbl(jLbl.I()));
+    assert CrashTolerantJournal.Next(I(v), I(v'), IALabel(lbl));
+  }
+
+  lemma NextRefines(v: Variables, v': Variables, lbl: TransitionLabel)
+    requires Inv(v)
+    requires Next(v, v', lbl)
+    ensures Inv(v')
+    ensures CrashTolerantJournal.Next(I(v), I(v'), IALabel(lbl))
+  {
+    match lbl.base {
+      case LoadEphemeralFromPersistentLabel() =>
+        // Done
+        LoadEphemeralFromPersistentRefines(v, v', lbl);
+        assert Inv(v');
+        assert CrashTolerantJournal.Next(I(v), I(v'), IALabel(lbl));
+      case ReadForRecoveryLabel(_) => 
+        // Done
+        ReadForRecoveryRefines(v, v', lbl);
+        assert Inv(v');
+        assert CrashTolerantJournal.Next(I(v), I(v'), IALabel(lbl));
+      case QueryEndLsnLabel(_) => 
+        assume false;
+        assert Inv(v');
+        assert CrashTolerantJournal.Next(I(v), I(v'), IALabel(lbl));
+      case PutLabel(_) =>
+        assume false;
+        // assert Inv(v');
+        // assert CrashTolerantJournal.Next(I(v), I(v'), IALabel(lbl));
+      case InternalLabel() => 
+        assume false;
+        // assert Inv(v');
+        // assert CrashTolerantJournal.Next(I(v), I(v'), IALabel(lbl));
+      case QueryLsnPersistenceLabel(_) => 
+        assume false;
+        // assert Inv(v');
+        // assert CrashTolerantJournal.Next(I(v), I(v'), IALabel(lbl));
+      case CommitStartLabel(_, _) => 
+        assume false;
+        // assert Inv(v');
+        // assert CrashTolerantJournal.Next(I(v), I(v'), IALabel(lbl));
+      case CommitCompleteLabel(_) => 
+        assume false;
+        // assert Inv(v');
+        // assert CrashTolerantJournal.Next(I(v), I(v'), IALabel(lbl));
+      case CrashLabel() => 
+        assume false;
+        // assert Inv(v');
+        // assert CrashTolerantJournal.Next(I(v), I(v'), IALabel(lbl));
+    }
+  }
+
+
+
+
+}
+
